preuve presque finie :-)
git-svn-id: https://www.lri.fr/svn/demons/why2/trunk@555 ecafba89-7d34-45a1-8a0b-92829e960b72

examples/binary-search-c/bsearch.c
@@ -1,17 +1,17 @@
 
-/*W logic In : int array,int,int -> prop */
+/*W logic In : int array,int,int,int -> prop */
 
 int binary_search(int t[], int n, int v) 
 /*@ array_length(t) = n and n >= 0 and sorted_array(t,0,n-1) */
 {
   int l,u,p,m;
-  l = 1; 
+  l = 0; 
   u = n-1; 
   p = -1;
   while (l <= u) 
     /*@ invariant 
 	  0 <= l and u <= array_length(t)-1 and -1 <= p <= array_length(t)-1
-          and (p = -1 -> In(t,0,array_length(t)-1) -> In(t,l,u))
+          and (p = -1 -> In(t,0,array_length(t)-1,v) -> In(t,l,u,v))
           and (p >= 0 -> t[p]=v)
         variant 2+u-l */ {
     m = (l + u) / 2;
@@ -26,6 +26,6 @@ int binary_search(int t[], int n, int v)
   return -1;
 }
 /*@ (0 <= result <= array_length(t)-1 and t[result]=v) or 
-    (result = -1 and not In(t,1,array_length(t)-1)) */
+    (result = -1 and not In(t,1,array_length(t)-1,v)) */
 
 
